$$\Gamma = AT(L-L_0)$$
$$A, C_{L}, L_{1}\to L_f$$

## a) $(\Delta T)_S$

$$dS = \left(\frac{\partial S}{\partial T}\right)_{L}dT + \left(\frac{\partial S}{\partial L}\right)_{T}dL$$

$$T dS = C_{L}dT - T \left(\frac{\partial\Gamma}{\partial T}\right)_{L}dL$$
Since we want an adiabatic situation, $dS =0$ and thus:
$$C_{L}dT =  T \left(\frac{\partial\Gamma}{\partial T}\right)_{L}dL$$
$$\frac{dT}{T}=  \int\frac{\left(\frac{\partial\Gamma}{\partial T}\right)_{L}}{C_{L}}dL$$
That is,
$$T_{f}= T_{i}e^{A \frac{(L-L_{0})^{2}}{2C_{L}}}$$
## b) $\Delta U$

$$\Delta U = W_{i\to f} = \int_{L_{i}}^{L_{f}}\Gamma dL = \int_{L_{i}}^{L_{f}} A T (L-L_0)dL$$

But do not be mistaken: $T$ is a function of $L$. Let's put it there:

$$\Delta U = \int_{L_{i}}^{L_{f}} A T_ie^{A \frac{(L-L_{0})^{2}}{2C_{L}}} (L-L_{0)dL}= C_{L}T_{i}\left[e^{\frac{A(L_{f} - L_{i})^{2}}{2C_{L}}}-1\right]=C_L(T_{f}-T_i)$$


## c) $\Delta S$
It is an adiabatic process, thus $\Delta S =0$

## d) $\Delta H$, $\Delta F$, $\Delta G$

In this case;

$$H = U -\Gamma L = H(S,\Gamma)$$

$$F = U -TS = F(T,L)$$

$$G = U - TS - \Gamma L = G(T, \Gamma)$$

So, we have that:
$$(\Delta H)_S = \Delta U - \Gamma \Delta L - L \Delta\Gamma = \Delta U -\Gamma_fL_{f}+\Gamma_iL_{i} = \Delta U -ATL_{f}(L_f-L_{0})$$ 

$$(\Delta F)_{S}=\Delta U - S\Delta T  $$

$$(\Delta G )_{S} =\Delta H -S\Delta T $$